Make safechecker compute (#682)
* make eqb compute

* change some Qed's to Defined

* test file

* Fix definition of equality of terms, contexts etc in PCUIC to be efficient and transparent

* add fuel to isconf_full and fix other computation issues

* correct ReflectEq for case_info

* remove useless and dangerous instance of EqDec_ReflectEq

* more uniform treatment of Reflect

* make recursive calls compute in SafeConversion

* clean up computational content

* make guard compute

* typecheck_program build the environement

* add more tests in test-suite

* fix plugin generation

* more computation

* add missing import

Co-authored-by: Matthieu Sozeau <mattam@mattam.org>

safechecker/theories/SafeTemplateChecker.v
@@ -12,12 +12,17 @@ Definition trans_program (p : Ast.Env.program) : program :=
   let Σ' := trans_global_env p.1 in
   (Σ', trans Σ' p.2).
 
+Definition EnvCheck_wf_env_ext {cf:checker_flags} := EnvCheck wf_env_ext. 
+
+Local Instance Monad_EnvCheck_wf_env_ext {cf:checker_flags} : Monad EnvCheck_wf_env_ext := _.
+
 Program Definition infer_template_program {cf : checker_flags} {nor : normalizing_flags} (p : Ast.Env.program) φ
-  : EnvCheck wf_env_ext (let p' := trans_program p in ∑ A, ∥ (p'.1, φ) ;;; [] |- p'.2 : A ∥) :=
-  p <- typecheck_program optimized_abstract_env_impl (trans_program p) φ ;;
-  ret (p.π1 ; _).
-Next Obligation.
-  sq. destruct X. eapply infering_typing; tea. eapply w. constructor.
+  : EnvCheck_wf_env_ext (let p' := trans_program p in ∑ A, { X : wf_env_ext |
+    ∥ (p'.1, φ) = X.(wf_env_ext_referenced).(referenced_impl_env_ext) × wf_ext (p'.1, φ) ×  (p'.1, φ) ;;; [] |- p'.2 : A ∥ }) :=
+  pp <- typecheck_program (cf := cf) optimized_abstract_env_impl (trans_program p) φ ;;
+  ret (pp.π1 ; (exist (proj1_sig pp.π2) _)).
+Next Obligation. 
+  sq. destruct H; split; eauto. destruct p0; split; eauto.  eapply infering_typing; tea. eapply w. constructor.
 Qed.
 
 Program Definition infer_and_print_template_program {cf : checker_flags} {nor : normalizing_flags} (p : Ast.Env.program) φ
